first try at new types

verif/btrees/btrees.v
@@ -63,99 +63,134 @@ Qed.
 Variable X:Type.                (* val or unit *)
 
 (* Btree Types *)
-Inductive entry (X:Type): Type :=
-     | keyval: key -> V -> X -> entry X
-     | keychild: key -> node X -> entry X
-with node (X:Type): Type :=
-     | btnode: option (node X) -> listentry X -> bool -> bool -> bool -> X -> node X
-with listentry (X:Type): Type :=
-     | nil: listentry X
-     | cons: entry X -> listentry X -> listentry X.
 
-Definition cursor (X:Type): Type := list (node X * index). (* ancestors and index *)
-Definition relation (X:Type): Type := node X * X.  (* root and address *)
+(* Augmented BTree Type *)
+(* If X is val, we remember the address of each structure *)
+Inductive aentry (X:Type): Type :=
+     | keyval: key -> V -> X -> aentry X
+     | keychild: key -> anode X -> aentry X
+with anode (X:Type): Type :=
+     | btnode: option (anode X) -> alistentry X -> bool -> bool -> bool -> X -> anode X
+with alistentry (X:Type): Type :=
+     | nil: alistentry X
+     | cons: aentry X -> alistentry X -> alistentry X.
+
+(* Formal BTree Type *)
+Definition entry : Type := aentry unit.
+Definition node : Type := anode unit.
+Definition listentry : Type := alistentry unit.
+
+(* Transform an augmented tree into a formal one *)
+Fixpoint formalize (X:Type) (an:anode X) : node :=
+  match an with
+  | btnode o le isleaf first last x =>
+    match o with
+    | None => btnode unit None (formalize_le X le) isleaf first last tt
+    | Some n => btnode unit (Some (formalize X n)) (formalize_le X le) isleaf first last tt
+    end
+  end
+with formalize_le (X:Type) (ale:alistentry X) : listentry :=
+       match ale with
+       | nil => nil unit
+       | cons e le => cons unit (formalize_entry X e) (formalize_le X le)
+       end
+with formalize_entry (X:Type) (e: aentry X) : entry :=
+       match e with
+       | keyval k v x => keyval unit k v tt
+       | keychild k c => keychild unit k (formalize X c)
+       end.
+
+Definition acursor (X:Type): Type := list (anode X * index). (* ancestors and index *)
+Definition arelation (X:Type): Type := anode X * X.  (* root and address *)
+Definition cursor : Type := acursor unit.
+Definition relation : Type := arelation unit.
+
+Definition formalize_rel (X:Type) (ar: arelation X) : relation :=
+  match ar with
+    (an,prel) => (formalize X an,tt)
+  end.
 
 (* Btrees depth *)
-Fixpoint node_depth {X:Type} (n:node X) : nat :=
+Fixpoint node_depth {X:Type} (n:anode X) : nat :=
   match n with
     btnode ptr0 le _ _ _ _ => max_nat (listentry_depth le)
                                 (match ptr0 with
                                  | None => O
                                  | Some n' => S (node_depth n') end)
   end
-with listentry_depth {X:Type} (le:listentry X) : nat :=
+with listentry_depth {X:Type} (le:alistentry X) : nat :=
        match le with
        | nil => O
        | cons e le' => max_nat (entry_depth e) (listentry_depth le')
        end
-with entry_depth {X:Type} (e:entry X) : nat :=
+with entry_depth {X:Type} (e:aentry X) : nat :=
        match e with
        | keyval _ _ _ => O
        | keychild _ n => S (node_depth n)
        end.
 
 (* root of the relation *)
-Definition get_root {X:Type} (rel:relation X) : node X := fst rel.
+Definition get_root {X:Type} (rel:arelation X) : anode X := fst rel.
 
 (* cursor depth used for putentry. the entry_depth should be equal the cursor depth *)
-Definition cursor_depth {X:Type} (c:cursor X) (r:relation X) : nat :=
+Definition cursor_depth {X:Type} (c:acursor X) (r:arelation X) : nat :=
   match c with
   | [] => S (node_depth (get_root r))
   | (n,i)::c' => node_depth n
   end.
 
 (* Number of Records *)
-Fixpoint node_numrec {X:Type} (n:node X) : nat :=
+Fixpoint node_numrec {X:Type} (n:anode X) : nat :=
   match n with
     btnode ptr0 le _ _ _ _ => listentry_numrec le + match ptr0 with
                                                    | None => O
                                                    | Some n' => node_numrec n'
                                                    end
   end
-with listentry_numrec {X:Type} (le:listentry X) : nat :=
+with listentry_numrec {X:Type} (le:alistentry X) : nat :=
        match le with
        | nil => O
        | cons e le' => entry_numrec e + listentry_numrec le'
        end
-with entry_numrec {X:Type} (e:entry X) : nat :=
+with entry_numrec {X:Type} (e:aentry X) : nat :=
        match e with
        | keyval _ _ _ => S O
        | keychild _ n => node_numrec n
        end.         
 
 (* numRecords of the relation *)
-Definition get_numrec {X:Type} (rel:relation X) : nat := node_numrec (get_root rel).
+Definition get_numrec {X:Type} (rel:arelation X) : nat := node_numrec (get_root rel).
 
 (* depth of the relation *)
-Definition get_depth {X:Type} (rel:relation X) : nat := node_depth (get_root rel).
+Definition get_depth {X:Type} (rel:arelation X) : nat := node_depth (get_root rel).
   
 (* Index at the current level *)
-Definition entryIndex {X:Type} (c:cursor X) : index :=
+Definition entryIndex {X:Type} (c:acursor X) : index :=
   match c with
   | [] => ip 0
   | (n,i)::c' => i
   end.
 
 (* Ancestor at the current level *)
-Definition currNode {X:Type} (c:cursor X) (r:relation X) : node X :=
+Definition currNode {X:Type} (c:acursor X) (r:arelation X) : anode X :=
   match c with
   | [] => get_root r
   | (n,i)::c' => n
   end.
 
 (* number of keys in a listentry *)
-Fixpoint numKeys_le {X:Type} (le:listentry X) : nat :=
+Fixpoint numKeys_le {X:Type} (le:alistentry X) : nat :=
   match le with
   | nil => O
   | cons _ le' => S (numKeys_le le')
   end.
 
-(* number of keys in a node *)
-Definition numKeys {X:Type} (n:node X) : nat :=
+(* number of keys in a anode *)
+Definition numKeys {X:Type} (n:anode X) : nat :=
   match n with btnode ptr0 le _ _ _ x => numKeys_le le end.
 
 (* is a cursor valid? invalid if the cursor is past the very last key *)
-Definition isValid {X:Type} (c:cursor X) (r:relation X): bool :=
+Definition isValid {X:Type} (c:acursor X) (r:arelation X): bool :=
   match currNode c r
   with btnode ptr0 le b First Last x =>
        match Last with
@@ -169,7 +204,7 @@ Definition isValid {X:Type} (c:cursor X) (r:relation X): bool :=
   end.
 
 (* does the cursor point to the very first key? *)
-Definition isFirst {X:Type} (c:cursor X) : bool :=
+Definition isFirst {X:Type} (c:acursor X) : bool :=
   match c with
   | [] => false
   | (n,i)::c' =>
@@ -179,7 +214,7 @@ Definition isFirst {X:Type} (c:cursor X) : bool :=
   end.
 
 (* Is a given node a leaf node *)
-Definition LeafNode {X:Type} (n:node X) : Prop :=
+Definition LeafNode {X:Type} (n:anode X) : Prop :=
   match n with btnode _ _ b _ _ _ =>
                match b with
                | true => True
@@ -188,7 +223,7 @@ Definition LeafNode {X:Type} (n:node X) : Prop :=
   end.
 
 (* Is a given node an intern node *)
-Definition InternNode {X:Type} (n:node X) : Prop :=
+Definition InternNode {X:Type} (n:anode X) : Prop :=
   match n with btnode _ _ b _ _ _ =>
                match b with
                | true => False
@@ -197,14 +232,14 @@ Definition InternNode {X:Type} (n:node X) : Prop :=
   end.
 
 (* Leaf entries have values *)
-Definition LeafEntry {X:Type} (e:entry X) : Prop :=
+Definition LeafEntry {X:Type} (e:aentry X) : Prop :=
   match e with
   | keyval _ _ _ => True
   | keychild _ _ => False
   end.
 
 (* nth entry of a listentry *)
-Fixpoint nth_entry_le {X:Type} (i:nat) (le:listentry X): option (entry X) :=
+Fixpoint nth_entry_le {X:Type} (i:nat) (le:alistentry X): option (aentry X) :=
   match i with
   | O => match le with
          | nil => None
@@ -216,7 +251,7 @@ Fixpoint nth_entry_le {X:Type} (i:nat) (le:listentry X): option (entry X) :=
             end
   end.
 
-Lemma nth_entry_le_some : forall (X:Type) (le:listentry X) i e,
+Lemma nth_entry_le_some : forall (X:Type) (le:alistentry X) i e,
     nth_entry_le i le = Some e -> (i < numKeys_le le)%nat.
 Proof.
   intros. generalize dependent le.
@@ -227,7 +262,7 @@ Proof.
   - simpl in H. apply IHi in H. simpl. omega.
 Qed.
 
-Lemma nth_entry_le_in_range: forall (X:Type) i (le:listentry X),
+Lemma nth_entry_le_in_range: forall (X:Type) i (le:alistentry X),
     (i < numKeys_le le)%nat ->
     exists e, nth_entry_le i le = Some e.
 Proof.
@@ -235,22 +270,22 @@ Proof.
   induction le.
   - intros. simpl in H. omega.
   - intros. destruct i.
-    + simpl. exists e. auto.
+    + simpl. exists a. auto.
     + simpl. apply IHle. simpl in H. omega.
 Qed.
 
 (* nth entry of a node *)
-Definition nth_entry {X:Type} (i:nat) (n:node X): option (entry X) :=
+Definition nth_entry {X:Type} (i:nat) (n:anode X): option (aentry X) :=
   match n with btnode ptr0 le b First Last x => nth_entry_le i le end.
 
-Lemma nth_entry_some : forall (X:Type) (n:node X) i e,
+Lemma nth_entry_some : forall (X:Type) (n:anode X) i e,
     nth_entry i n = Some e ->  (i < numKeys n)%nat.
 Proof.
   intros. unfold nth_entry in H. destruct n. apply nth_entry_le_some in H. simpl. auto.
 Qed.
 
 (* nth child of a listentry *)
-Fixpoint nth_node_le {X:Type} (i:nat) (le:listentry X): option (node X) :=
+Fixpoint nth_node_le {X:Type} (i:nat) (le:alistentry X): option (anode X) :=
   match i with
   | O => match le with
          | nil => None
@@ -277,7 +312,7 @@ Proof.
     + simpl. simpl in H. apply IHle in H. auto.
 Qed.
 
-Lemma nth_node_le_some : forall (X:Type) (le:listentry X) i n,
+Lemma nth_node_le_some : forall (X:Type) (le:alistentry X) i n,
     nth_node_le i le = Some n -> (i < numKeys_le le)%nat.
 Proof.
   intros. generalize dependent le.
@@ -286,7 +321,7 @@ Proof.
   - destruct le. inv H. simpl in H. apply IHi in H. simpl. omega.
 Qed.
     
-Lemma nth_node_le_decrease: forall X (le:listentry X) (n:node X) i,
+Lemma nth_node_le_decrease: forall X (le:alistentry X) (n:anode X) i,
     nth_node_le i le = Some n ->
     (node_depth n < listentry_depth le)%nat.
 Proof.
@@ -295,12 +330,12 @@ Proof.
     destruct i; inversion H.
   - simpl.
     destruct i.
-    + apply le_max_split_l. simpl in H. destruct e; try inv H. simpl. auto.
+    + apply le_max_split_l. simpl in H. destruct a; try inv H. simpl. auto.
     + apply le_max_split_r. apply IHle with (i:=i). simpl in H. auto.
 Qed.
 
 (* nth child of a node *)
-Definition nth_node {X:Type} (i:index) (n:node X): option (node X) :=
+Definition nth_node {X:Type} (i:index) (n:anode X): option (anode X) :=
   match n with btnode ptr0 le _ _ _ _ =>
                match i with
                | im => ptr0
@@ -308,7 +343,7 @@ Definition nth_node {X:Type} (i:index) (n:node X): option (node X) :=
                end
   end.
 
-Lemma nth_node_some: forall (X:Type) (n:node X) i n',
+Lemma nth_node_some: forall (X:Type) (n:anode X) i n',
     nth_node i n = Some n' -> idx_to_Z i < Z.of_nat(numKeys n).
 Proof.
   intros.
@@ -317,7 +352,7 @@ Proof.
   - simpl. apply nth_node_le_some in H. omega.
 Qed.
 
-Lemma nth_node_decrease: forall X (n:node X) (n':node X) i,
+Lemma nth_node_decrease: forall X (n:anode X) (n':anode X) i,
     nth_node i n = Some n' ->
     (node_depth n' < node_depth n)%nat.
 Proof.
@@ -329,14 +364,14 @@ Proof.
 Qed.
 
 (* the node that the cursor points to *)
-Definition next_node {X:Type} (c:cursor X) (root:node X) : option (node X) :=
+Definition next_node {X:Type} (c:acursor X) (root:anode X) : option (anode X) :=
   match c with
   | [] => Some root
   | (n,i)::c' => nth_node i n
   end.    
 
 (* entry pointed to by a cursor. Leaf entry for a complete cursor. Keychild entry for a partial cursor *)
-Definition getCEntry {X:Type} (c:cursor X) : option (entry X) :=
+Definition getCEntry {X:Type} (c:acursor X) : option (aentry X) :=
   match c with
   | [] => None
   | (n,i)::c' =>
@@ -347,7 +382,7 @@ Definition getCEntry {X:Type} (c:cursor X) : option (entry X) :=
   end.
 
 (* get Key pointed to by cursor *)
-Definition getCKey {X:Type} (c:cursor X) : option key :=
+Definition getCKey {X:Type} (c:acursor X) : option key :=
   match (getCEntry c) with
   | None => None
   | Some e => match e with
@@ -357,7 +392,7 @@ Definition getCKey {X:Type} (c:cursor X) : option key :=
   end.
 
 (* get record pointed to by cursor *)
-Definition getCRecord {X:Type} (c:cursor X) : option V  :=
+Definition getCRecord {X:Type} (c:acursor X) : option V  :=
   match (getCEntry c) with
   | None => None
   | Some e => match e with
@@ -367,7 +402,7 @@ Definition getCRecord {X:Type} (c:cursor X) : option V  :=
   end.
 
 (* get address pointed to by cursor *)
-Definition getCVal {X:Type} (c:cursor X) : option X :=
+Definition getCVal {X:Type} (c:acursor X) : option X :=
   match (getCEntry c) with
   | None => None
   | Some e => match e with
@@ -377,7 +412,7 @@ Definition getCVal {X:Type} (c:cursor X) : option X :=
   end.
 
 (* findChildIndex for an intern node *)
-Fixpoint findChildIndex' {X:Type} (le:listentry X) (key:key) (i:index): index :=
+Fixpoint findChildIndex' {X:Type} (le:alistentry X) (key:key) (i:index): index :=
   match le with
   | nil => i
   | cons e le' =>
@@ -395,12 +430,12 @@ Fixpoint findChildIndex' {X:Type} (le:listentry X) (key:key) (i:index): index :=
     end
   end.
 
-Definition findChildIndex {X:Type} (n:node X) (key:key): index :=
+Definition findChildIndex {X:Type} (n:anode X) (key:key): index :=
   match n with btnode ptr0 le b F L x =>
                findChildIndex' le key im end.
 
 (* findRecordIndex for a leaf node *)
-Fixpoint findRecordIndex' {X:Type} (le:listentry X) (key:key) (i:index): index :=
+Fixpoint findRecordIndex' {X:Type} (le:alistentry X) (key:key) (i:index): index :=
   match le with
   | nil => i
   | cons e le' =>
@@ -418,12 +453,12 @@ Fixpoint findRecordIndex' {X:Type} (le:listentry X) (key:key) (i:index): index :
     end
   end.
 
-Definition findRecordIndex {X:Type} (n:node X) (key:key) : index :=
+Definition findRecordIndex {X:Type} (n:anode X) (key:key) : index :=
     match n with btnode ptr0 le b F L x =>
                  findRecordIndex' le key (ip O) end.
 
 (* nth key of a listentry *)
-Fixpoint nth_key {X:Type} (i:nat) (le:listentry X): option key :=
+Fixpoint nth_key {X:Type} (i:nat) (le:alistentry X): option key :=
   match le with
   | nil => None
   | cons e le' => match i with
@@ -436,7 +471,7 @@ Fixpoint nth_key {X:Type} (i:nat) (le:listentry X): option key :=
   end.
 
 (* takes a PARTIAL cursor, n next node (pointed to by the cursor) and goes down to first key *)
-Fixpoint moveToFirst {X:Type} (n:node X) (c:cursor X) (level:nat): cursor X :=
+Fixpoint moveToFirst {X:Type} (n:anode X) (c:acursor X) (level:nat): acursor X :=
   match n with
     btnode ptr0 le isLeaf First Last x =>
     match isLeaf with
@@ -449,7 +484,7 @@ Fixpoint moveToFirst {X:Type} (n:node X) (c:cursor X) (level:nat): cursor X :=
   end.
 
 (* takes a PARTIAL cursor, n next node (pointed to by the cursor) and goes down to last key *)
-Function moveToLast {X:Type} (n:node X) (c:cursor X) (level:nat) {measure node_depth n}: cursor X :=
+Function moveToLast {X:Type} (n:anode X) (c:acursor X) (level:nat) {measure node_depth n}: acursor X :=
   match n with
     btnode ptr0 le isLeaf First Last x =>
     match isLeaf with
@@ -465,7 +500,7 @@ Proof.
 Qed.
 
 (* takes a PARTIAL cursor, n next node (pointed to by the cursor) and goes down to the key, or where it should be inserted *)
-Function moveToKey {X:Type} (n:node X) (key:key) (c:cursor X) {measure node_depth n} : cursor X :=
+Function moveToKey {X:Type} (n:anode X) (key:key) (c:acursor X) {measure node_depth n} : acursor X :=
   match n with
     btnode ptr0 le isLeaf First Last x =>
     match isLeaf with
@@ -481,25 +516,25 @@ Proof.
 Qed.
 
 (* Returns node->isLeaf *)
-Definition isnodeleaf {X:Type} (n:node X) : bool :=
+Definition isnodeleaf {X:Type} (n:anode X) : bool :=
   match n with btnode _ _ isLeaf _ _ _ => isLeaf end.
 
 (* The key of an entry *)
-Definition entry_key {X:Type} (e:entry X) : key :=
+Definition entry_key {X:Type} (e:aentry X) : key :=
   match e with
   | keychild k c => k
   | keyval k v x => k
   end.
 
 (* Child of an entry *)
-Definition entry_child {X:Type} (e:entry X) : option (node X) :=
+Definition entry_child {X:Type} (e:aentry X) : option (anode X) :=
   match e with
   | keychild k c => Some c
   | keyval k v x => None
   end.
 
 (* Returns true if we know for sure that the node is a parent of the key *)
-Definition isNodeParent {X:Type} (n:node X) (key:key): bool :=
+Definition isNodeParent {X:Type} (n:anode X) (key:key): bool :=
   match n with btnode ptr0 le isLeaf First Last x =>
   match isLeaf with
   | true =>
@@ -529,7 +564,7 @@ Definition isNodeParent {X:Type} (n:node X) (key:key): bool :=
   end.
 
 (* Ascend to parent in a cursor *)
-Fixpoint AscendToParent {X:Type} (c:cursor X) (key:key): cursor X :=
+Fixpoint AscendToParent {X:Type} (c:acursor X) (key:key): acursor X :=
   match c with
   | [] => []
   | [(n,i)] => [(n,i)]          (* root is parent *)
@@ -540,7 +575,7 @@ Fixpoint AscendToParent {X:Type} (c:cursor X) (key:key): cursor X :=
   end.
 
 (* go to a Key from any position in the cursor: ascendtoparent then movetokey *)
-Definition goToKey {X:Type} (c:cursor X) (r:relation X) (key:key) : cursor X :=
+Definition goToKey {X:Type} (c:acursor X) (r:arelation X) (key:key) : acursor X :=
   let partialc := AscendToParent c key in
   match partialc with
   | [] => moveToKey X (get_root r) key []
@@ -548,7 +583,7 @@ Definition goToKey {X:Type} (c:cursor X) (r:relation X) (key:key) : cursor X :=
   end.
 
 (* Returns the index of the last pointer of a node *)
-Definition lastpointer {X:Type} (n:node X): index :=
+Definition lastpointer {X:Type} (n:anode X): index :=
   match n with btnode ptr0 le isLeaf First Last pn =>
                match isLeaf with
                | true => ip (numKeys_le le)
@@ -560,7 +595,7 @@ Definition lastpointer {X:Type} (n:node X): index :=
   end.
 
 (* Returns the index of the first pointer of a node *)
-Definition firstpointer {X:Type} (n:node X): index :=
+Definition firstpointer {X:Type} (n:anode X): index :=
   match n with btnode ptr0 le isLeaf First Last pn =>
                match isLeaf with
                | true => ip O
@@ -569,7 +604,7 @@ Definition firstpointer {X:Type} (n:node X): index :=
   end.
 
 (* Goes up in the cursor as long as the index is the last possible one for the current node *)
-Fixpoint up_at_last {X:Type} (c:cursor X): cursor X :=
+Fixpoint up_at_last {X:Type} (c:acursor X): acursor X :=
   match c with
   | [] => []
   | [(n,i)] => [(n,i)]
@@ -580,7 +615,7 @@ Fixpoint up_at_last {X:Type} (c:cursor X): cursor X :=
   end.
 
 (* Increments current index of the cursor. The current index should not be the last possible one *)
-Definition next_cursor {X:Type} (c:cursor X): cursor X :=
+Definition next_cursor {X:Type} (c:acursor X): acursor X :=
   match c with
   | [] => []
   | (n,i)::c' => (n,next_index i)::c'
@@ -588,7 +623,7 @@ Definition next_cursor {X:Type} (c:cursor X): cursor X :=
 
 (* moves the cursor to the next position (possibly an equivalent one)
    takes a FULL cursor as input *)
-Definition moveToNext {X:Type} (c:cursor X) (r:relation X) : cursor X :=
+Definition moveToNext {X:Type} (c:acursor X) (r:arelation X) : acursor X :=
   match isValid c r with
   | false => c                (* invalid cursor: no change to the cursor *)
   | _ =>
@@ -609,7 +644,7 @@ Definition moveToNext {X:Type} (c:cursor X) (r:relation X) : cursor X :=
   end.
 
 (* Goes up in the cursor as long as the index is the first possible one for the current node *)
-Fixpoint up_at_first {X:Type} (c:cursor X): cursor X :=
+Fixpoint up_at_first {X:Type} (c:acursor X): acursor X :=
   match c with
   | [] => []
   | (n,i)::c' => match index_eqb i (firstpointer n) with
@@ -619,7 +654,7 @@ Fixpoint up_at_first {X:Type} (c:cursor X): cursor X :=
   end.
 
 (* Decrements current index of the cursor. The current index should not be the first possible one *)
-Definition prev_cursor {X:Type} (c:cursor X): cursor X :=
+Definition prev_cursor {X:Type} (c:acursor X): acursor X :=
   match c with
   | [] => []
   | (n,i)::c' => (n,prev_index i)::c'
@@ -627,7 +662,7 @@ Definition prev_cursor {X:Type} (c:cursor X): cursor X :=
 
 (* moves the cursor to the previous position (possibly an equivalent one) 
  takes a FULL cursor as input *)
-Definition moveToPrev {X:Type} (c:cursor X) (r:relation X) : cursor X :=
+Definition moveToPrev {X:Type} (c:acursor X) (r:arelation X) : acursor X :=
   match isFirst c with
   | true => c                (* first cursor: no change to the cursor *)
   | _ =>
@@ -647,7 +682,7 @@ Definition moveToPrev {X:Type} (c:cursor X) (r:relation X) : cursor X :=
     end
   end.
 
-Definition normalize {X:Type} (c:cursor X) (r:relation X) : cursor X :=
+Definition normalize {X:Type} (c:acursor X) (r:arelation X) : acursor X :=
   match c with
   | [] => c
   | (n,i)::c' => match (index_eqb i (ip (numKeys n))) with
@@ -658,7 +693,7 @@ Definition normalize {X:Type} (c:cursor X) (r:relation X) : cursor X :=
 
 (* moves the cursor to the next non-equivalent position 
  takes a FULL cursor as input *)
-Definition RL_MoveToNext {X:Type} (c:cursor X) (r:relation X) : cursor X :=
+Definition RL_MoveToNext {X:Type} (c:acursor X) (r:arelation X) : acursor X :=
   match c with
   | [] => c                     (* not possible *)
   | (n,i)::c' => match (index_eqb i (ip (numKeys n))) with
@@ -669,7 +704,7 @@ Definition RL_MoveToNext {X:Type} (c:cursor X) (r:relation X) : cursor X :=
 
 (* move the cursor to the previous non-equivalent position 
  takes a FULL cursor as input *)
-Definition RL_MoveToPrevious {X:Type} (c:cursor X) (r:relation X) : cursor X :=
+Definition RL_MoveToPrevious {X:Type} (c:acursor X) (r:arelation X) : acursor X :=
   match c with
   | [] => c                     (* not possible *)
   | (n,i)::c => match (index_eqb i (ip O)) with
@@ -679,7 +714,7 @@ Definition RL_MoveToPrevious {X:Type} (c:cursor X) (r:relation X) : cursor X :=
   end.
 
 (* the nth first entries of a listentry *)
-Fixpoint nth_first_le {X:Type} (le:listentry X) (i:nat) {struct i}: listentry X :=
+Fixpoint nth_first_le {X:Type} (le:alistentry X) (i:nat) {struct i}: alistentry X :=
   match i with
   | O => nil X
   | S ii => match le with
@@ -689,7 +724,7 @@ Fixpoint nth_first_le {X:Type} (le:listentry X) (i:nat) {struct i}: listentry X 
   end.
 
 (* number of first keys *)
-Lemma numKeys_nth_first: forall (X:Type) (le:listentry X) i,
+Lemma numKeys_nth_first: forall (X:Type) (le:alistentry X) i,
     (i <= numKeys_le le)%nat ->
     numKeys_le (nth_first_le le i) = i.
 Proof.
@@ -702,7 +737,7 @@ Proof.
 Qed.
 
 (* selecting all keys of a listentry *)
-Lemma nth_first_same: forall X (l:listentry X) m,
+Lemma nth_first_same: forall X (l:alistentry X) m,
     m = numKeys_le l ->
     nth_first_le l m = l.
 Proof.
@@ -713,7 +748,7 @@ Proof.
 Qed.
 
 (* skips the nth first entries of a listentry *)
-Fixpoint skipn_le {X:Type} (le:listentry X) (i:nat) : listentry X :=
+Fixpoint skipn_le {X:Type} (le:alistentry X) (i:nat) : alistentry X :=
   match i with
   | O => le
   | S ii => match le with
@@ -723,7 +758,7 @@ Fixpoint skipn_le {X:Type} (le:listentry X) (i:nat) : listentry X :=
   end.
 
 (* number of keys when skipping *)
-Lemma numKeys_le_skipn: forall X (l:listentry X) m,
+Lemma numKeys_le_skipn: forall X (l:alistentry X) m,
     numKeys_le (skipn_le l m) = (numKeys_le l - m)%nat.
 Proof.
   intros. generalize dependent m.
@@ -733,16 +768,16 @@ Proof.
 Qed.
 
 (* sublist of a listentry *)
-Definition suble {X:Type} (lo hi: nat) (le:listentry X) : listentry X :=
+Definition suble {X:Type} (lo hi: nat) (le:alistentry X) : alistentry X :=
   nth_first_le (skipn_le le lo) (hi-lo).
 
-Lemma suble_nil: forall X (le:listentry X) lo,
+Lemma suble_nil: forall X (le:alistentry X) lo,
     suble lo lo le = nil X.
 Proof.
   intros. unfold suble. replace ((lo - lo)%nat) with O by omega. simpl. auto.
 Qed.
 
-Lemma suble_skip: forall A m f (l:listentry A),
+Lemma suble_skip: forall A m f (l:alistentry A),
     f = numKeys_le l -> 
     suble m f l = skipn_le l m.
 Proof.
@@ -751,14 +786,14 @@ Proof.
 Qed.
 
 (* appending two listentries *)
-Fixpoint le_app {X:Type} (l1:listentry X) (l2:listentry X) :=
+Fixpoint le_app {X:Type} (l1:alistentry X) (l2:alistentry X) :=
   match l1 with
   | nil => l2
   | cons e le => cons X e (le_app le l2)
   end.
 
 (* Inserts an entry in a list of entries (that doesnt already has the key) *)
-Fixpoint insert_le {X:Type} (le:listentry X) (e:entry X) : listentry X :=
+Fixpoint insert_le {X:Type} (le:alistentry X) (e:aentry X) : alistentry X :=
   match le with
   | nil => cons X e (nil X)
   | cons e' le' => match ((entry_key e).(k_) <=? (entry_key e').(k_)) with
@@ -768,19 +803,19 @@ Fixpoint insert_le {X:Type} (le:listentry X) (e:entry X) : listentry X :=
   end.
 
 (* inserting adds one entry *)
-Lemma numKeys_le_insert: forall X (l:listentry X) e,
+Lemma numKeys_le_insert: forall X (l:alistentry X) e,
     numKeys_le (insert_le l e) = S (numKeys_le l).
 Proof.
   intros. induction l.
   - simpl. auto.
-  - simpl. destruct (k_ (entry_key e) <=? k_ (entry_key e0)).
+  - simpl. destruct (k_ (entry_key e) <=? k_ (entry_key a)).
     + simpl. auto.
     + simpl. rewrite IHl. auto.
 Qed.
 
 (* Inserts an entry e in a full node n. This function returns the right node containing the first 
    values after the split. e should have a key not already contained by the node *)
-Definition splitnode_left {X:Type} (n:node X) (e:entry X) : (node X) :=
+Definition splitnode_left {X:Type} (n:anode X) (e:aentry X) : (anode X) :=
   match n with btnode ptr0 le isLeaf First Last x =>
                btnode X ptr0
                       (nth_first_le (insert_le le e) Middle)
@@ -789,7 +824,7 @@ Definition splitnode_left {X:Type} (n:node X) (e:entry X) : (node X) :=
                       false    (* the right node can't be the last one *)
                       x end.
 
-Definition splitnode_leafnode {X:Type} (le:listentry X) (e:entry X) (newx:X) Last :=
+Definition splitnode_leafnode {X:Type} (le:alistentry X) (e:aentry X) (newx:X) Last :=
   (btnode X None (* Leaf node has no ptr0 *)
           (skipn_le (insert_le le e) Middle)
           true   (* newnode is at same level as old one *)
@@ -797,7 +832,7 @@ Definition splitnode_leafnode {X:Type} (le:listentry X) (e:entry X) (newx:X) Las
           Last   (* newnode is last leaf if the split node was *)
           newx).
 
-Definition splitnode_internnode {X:Type} (le:listentry X) (e:entry X) newx Last child :=
+Definition splitnode_internnode {X:Type} (le:alistentry X) (e:aentry X) newx Last child :=
   (btnode X (Some child) (* ptr0 of the new node is the previous child of the pushed up entry *)
           (skipn_le (insert_le le e) (S Middle)) (* the middle entry isn't copied *)
           false  (* newnode is at the same level as old one *)
@@ -808,7 +843,7 @@ Definition splitnode_internnode {X:Type} (le:listentry X) (e:entry X) newx Last 
 (* This function contains the new entry to be pushed up after splitting the node
    Its child is the new node from splinode, containing the last entries 
    newx is the the address of the new node *)
-Definition splitnode_right {X:Type} (n:node X) (e:entry X) (newx:X) : (entry X) :=
+Definition splitnode_right {X:Type} (n:anode X) (e:aentry X) (newx:X) : (aentry X) :=
   match n with
     btnode ptr0 le isLeaf First Last x =>
     match isLeaf with
@@ -833,7 +868,7 @@ Definition splitnode_right {X:Type} (n:node X) (e:entry X) (newx:X) : (entry X) 
   end.
 
 (* The key that is copied up when splitting a node *)
-Definition splitnode_key {X:Type} (n:node X) (e:entry X) : key :=
+Definition splitnode_key {X:Type} (n:anode X) (e:aentry X) : key :=
   match n with
     btnode ptr0 le isLeaf First Last x =>
     match nth_entry_le Middle (insert_le le e) with
@@ -847,11 +882,11 @@ Definition splitnode_key {X:Type} (n:node X) (e:entry X) : key :=
   end.
   
 (* returns true if the node is full and should be split on insertion *)
-Definition fullnode {X:Type} (n:node X) : bool :=
+Definition fullnode {X:Type} (n:anode X) : bool :=
   (Fanout <=? numKeys n)%nat.
 
 (* Is a key already in a listentry? *)
-Fixpoint key_in_le {X:Type} (key:key) (le:listentry X) : bool :=
+Fixpoint key_in_le {X:Type} (key:key) (le:alistentry X) : bool :=
   match le with
   | nil => false
   | cons e le' => match ((entry_key e).(k_) =? key.(k_)) with
@@ -863,7 +898,7 @@ Fixpoint key_in_le {X:Type} (key:key) (le:listentry X) : bool :=
 (* listentry should contain an entry with the same key as e
    the child or record of this entry will be updated to the one of the entry 
    this is useful when inserting a (key,record) in a tree where the key has already been inserted *)
-Fixpoint update_le {X:Type} (e:entry X) (le:listentry X) : listentry X :=
+Fixpoint update_le {X:Type} (e:aentry X) (le:alistentry X) : alistentry X :=
   match le with
   | nil => nil X                 (* not possible *)
   | cons e' le' => match ((entry_key e).(k_) =? (entry_key e').(k_)) with
@@ -873,7 +908,7 @@ Fixpoint update_le {X:Type} (e:entry X) (le:listentry X) : listentry X :=
   end.
 
 (* updates a child in a listentry *)
-Fixpoint update_le_nth_child {X:Type} (i:nat) (le:listentry X) (n:node X) : listentry X :=
+Fixpoint update_le_nth_child {X:Type} (i:nat) (le:alistentry X) (n:anode X) : alistentry X :=
   match le with
   | nil => nil X
   | cons e le' => match i with
@@ -886,7 +921,7 @@ Fixpoint update_le_nth_child {X:Type} (i:nat) (le:listentry X) (n:node X) : list
   end.  
 
 (* updates value in a listentry *)
-Fixpoint update_le_nth_val {X:Type} (i:nat) (le:listentry X) (newv:V) (newx:X) : listentry X :=
+Fixpoint update_le_nth_val {X:Type} (i:nat) (le:alistentry X) (newv:V) (newx:X) : alistentry X :=
   match le with
   | nil => nil X
   | cons e le' => match i with
@@ -899,7 +934,7 @@ Fixpoint update_le_nth_val {X:Type} (i:nat) (le:listentry X) (newv:V) (newx:X) :
   end.
 
 (* updates nth child of a node *)
-Definition update_node_nth_child {X:Type} (i:index) (oldn:node X) (n:node X) : node X :=
+Definition update_node_nth_child {X:Type} (i:index) (oldn:anode X) (n:anode X) : anode X :=
   match oldn with btnode ptr0 le isLeaf First Last x =>
   match i with
   | im => btnode X (Some n) le isLeaf First Last x
@@ -909,7 +944,7 @@ Definition update_node_nth_child {X:Type} (i:index) (oldn:node X) (n:node X) : n
 
 (* recursivey updates a cursor with a new leaf node *)
 (* DEPRECATED *)
-Fixpoint update_cursor {X:Type} (c:cursor X) (n:node X) : cursor X :=
+Fixpoint update_cursor {X:Type} (c:acursor X) (n:anode X) : acursor X :=
   match c with
   | [] => []
   | (oldn,i)::c' =>
@@ -919,7 +954,7 @@ Fixpoint update_cursor {X:Type} (c:cursor X) (n:node X) : cursor X :=
 
 (* recursively updates a partial cursor and the corresponding relation wih a new node (to be put where the cursor points to) 
    the new cursor will point to n *)
-Fixpoint update_partial_cursor_rel {X:Type} (c:cursor X) (r:relation X) (n:node X) : (cursor X * relation X) :=
+Fixpoint update_partial_cursor_rel {X:Type} (c:acursor X) (r:arelation X) (n:anode X) : (acursor X * arelation X) :=
   match r with (root,prel) =>
   match c with
   | [] => ([], (n,prel))
@@ -930,7 +965,7 @@ Fixpoint update_partial_cursor_rel {X:Type} (c:cursor X) (r:relation X) (n:node 
   end
   end.
 
-Lemma update_partial_same_length: forall X (c:cursor X) r n,
+Lemma update_partial_same_length: forall X (c:acursor X) r n,
     length c = length (fst (update_partial_cursor_rel c r n)).
 Proof.
   intros. destruct r as [root prel].
@@ -948,7 +983,7 @@ Qed.
 (* recursively updates a cursor and the relation with a new node (that should replace the currNode) 
    this need a non-empty cursor
    the index is unchanged. Should it be updated somehow?*)
-Definition update_currnode_cursor_rel {X:Type} (c:cursor X) (r:relation X) (n:node X) : (cursor X * relation X) :=
+Definition update_currnode_cursor_rel {X:Type} (c:acursor X) (r:arelation X) (n:anode X) : (acursor X * arelation X) :=
   match c with
   | [] => (c,r)                  (* impossible, we ask for a non-empty cursor *)
   | (oldn, i)::c' =>
@@ -956,7 +991,7 @@ Definition update_currnode_cursor_rel {X:Type} (c:cursor X) (r:relation X) (n:no
     ((n,i)::newc', newrel)
   end.
 
-Lemma update_currnode_same_length: forall X (c:cursor X) r n,
+Lemma update_currnode_same_length: forall X (c:acursor X) r n,
     length c = length (fst (update_currnode_cursor_rel c r n)).
 Proof.
   intros. destruct c as [|[n' i] c'].
@@ -972,7 +1007,7 @@ Qed.
    the cursor should point to where the entry has to be inserted
    newx is the addresses of the new nodes for splitnode. d is default value (shouldn't be used)
    we remember with oldk the key that was inserted in the tree: the cursor should point to it *)
-Function putEntry {X:Type} (c:cursor X) (r:relation X) (e:entry X) (oldk:key) (newx:list X) (d:X) {measure length c}: (cursor X * relation X) :=
+Function putEntry {X:Type} (c:acursor X) (r:arelation X) (e:aentry X) (oldk:key) (newx:list X) (d:X) {measure length c}: (acursor X * arelation X) :=
   match r with
     (root, prel) =>
     match c with
@@ -1045,14 +1080,14 @@ Qed.
 (* Add a new (key,record) in a btree, updating cursor and relation
    x is the address of the new entry to insert 
    newx is the list of addresses for the new nodes of splitnode *)
-Definition RL_PutRecord {X:Type} (c:cursor X) (r:relation X) (key:key) (record:V) (x:X) (newx:list X) (d:X) : (cursor X * relation X) :=
+Definition RL_PutRecord {X:Type} (c:acursor X) (r:arelation X) (key:key) (record:V) (x:X) (newx:list X) (d:X) : (acursor X * arelation X) :=
   let c' := goToKey c r key in
   let e := keyval X key record x in
   let (putc, putr) := putEntry X c' r e key newx d in
   (RL_MoveToNext putc putr, putr).
 
 (* Gets the record pointed to by the cursor *)
-Definition RL_GetRecord (c:cursor val) r : val :=
+Definition RL_GetRecord (c:acursor val) r : val :=
   let normc := normalize c r in
   match getCVal normc with
   | None => nullval
